examples/kv_parsing/ValidatedParser.fst
@@ -123,53 +123,6 @@ let parse_num_entries_valid input =
 // method to encode dependencies (luckily the length of a bslice can be accessed
 // without a heap).
 
-#reset-options "--z3rlimit 15"
-
-// TODO: this isn't a parser_st_nochk because its output isn't exactly the same
-// as the parser; the relationship requires converting the return value to bytes
-let parse_u16_array_nochk : input:bslice -> Stack (u16_array_st * off:U32.t{U32.v off <= U32.v input.len})
-  (requires (fun h0 -> live h0 input /\
-                    (let bs = as_seq h0 input in
-                    Some? (parse_u16_array bs))))
-  (ensures (fun h0 r h1 ->
-              live h1 input /\
-              modifies_none h0 h1 /\
-              (let bs = B.as_seq h1 input.p in
-                Some? (parse_u16_array bs) /\
-                (let (v, n) = Some?.v (parse_u16_array bs) in
-                  let (rv, off) = r in
-                  // BUG: ommitting this live assertion causes failure in the
-                  // precondition to as_u16_array, but the error reported is
-                  // simply "ill-kinded type" on as_u16_array
-                  live h1 rv.a16_st /\
-                  as_u16_array h1 rv == v /\
-                  n == U32.v off)))) = fun input ->
-  let (len, off) = parse_u16_st_nochk input in
-  let input = advance_slice input off in
-  let a = U16ArraySt len (truncate_slice input (Cast.uint16_to_uint32 len)) in
-  (a, U32.add off (Cast.uint16_to_uint32 len))
-
-#reset-options
-
-let parse_u32_array_nochk : input:bslice -> Stack (u32_array_st * off:U32.t)
-  (requires (fun h0 -> live h0 input /\
-                    (let bs = as_seq h0 input in
-                    Some? (parse_u32_array bs))))
-  (ensures (fun h0 r h1 ->
-              live h1 input /\
-              modifies_none h0 h1 /\
-              (let bs = B.as_seq h1 input.p in
-                Some? (parse_u32_array bs) /\
-                (let (v, n) = Some?.v (parse_u32_array bs) in
-                  let (rv, off) = r in
-                  live h1 rv.a32_st /\
-                  as_u32_array h1 rv == v /\
-                  n == U32.v off)))) = fun input ->
-  let (len, off) = parse_u32_st_nochk input in
-  let input = advance_slice input off in
-  let a = U32ArraySt len (truncate_slice input len) in
-  (a, U32.add off len)
-
 #reset-options "--z3rlimit 20"
 
 let parse_entry_st_nochk : input:bslice -> Stack (entry_st * off:U32.t{U32.v off <= U32.v input.len})
